basis/TimeProofScript.sml
@@ -1,0 +1,79 @@
+(*
+  Proof about the command-line module of the CakeML standard basis library.
+*)
+open preamble ml_translatorTheory ml_progLib ml_translatorLib cfLib
+     TimeProgTheory timeFFITheory Word8ArrayProofTheory cfMonadLib
+     Word8ProgTheory Word8ArrayProofTheory MarshallingProgTheory MarshallingTheory
+     integerTheory int_arithTheory;
+
+val _ = new_theory"TimeProof";
+
+val _ = translation_extends"TimeProg";
+
+Definition TIME_def:
+  TIME ts ⇔ IOx ts_ffi_part ts
+End
+
+val set_thm =
+  TIME_def
+  |> SIMP_RULE(srw_ss())[
+       cfHeapsBaseTheory.IOx_def,ts_ffi_part_def,
+       cfHeapsBaseTheory.IO_def, set_sepTheory.one_def ]
+  |> SIMP_RULE(srw_ss())[Once FUN_EQ_THM,
+        set_sepTheory.SEP_EXISTS_THM,set_sepTheory.cond_STAR,PULL_EXISTS]
+  |> Q.SPEC`ts`
+val set_tm = set_thm |> concl |> find_term(pred_setSyntax.is_insert);
+
+Theorem TIME_FFI_part_hprop:
+  FFI_part_hprop (TIME x)
+Proof
+  rw [TIME_def,cfHeapsBaseTheory.IO_def,cfMainTheory.FFI_part_hprop_def,
+      cfHeapsBaseTheory.IOx_def,ts_ffi_part_def,
+      set_sepTheory.SEP_CLAUSES,set_sepTheory.SEP_EXISTS_THM,
+      set_sepTheory.cond_STAR]
+  \\ fs[set_sepTheory.one_def]
+QED
+
+val eq_v_thm = fetch "mlbasicsProg" "eq_v_thm"
+val eq_word8_v_thm = MATCH_MP (DISCH_ALL eq_v_thm) (EqualityType_NUM_BOOL |> cj 4) |> INST_TYPE [“:'a” |-> “:8”]
+
+Theorem nowMilliseconds_spec:
+  ∀t d ds uv.
+     UNIT_TYPE () uv ⇒
+     (d+t) DIV 1000 ≤ 256**8 - 1⇒
+     app (p:'ffi ffi_proj) Time_nowMilliseconds_v [uv]
+         (TIME <| latest_time := t; microseconds_elapsed := d:::ds |>)
+         (POSTv v. &NUM ((t+d) DIV 1000) v * TIME <| latest_time := t+d; microseconds_elapsed := ds |>)
+Proof
+  xcf_with_def "Time.nowMilliseconds" Time_nowMilliseconds_v_def \\
+  xmatch \\
+  gvs[UNIT_TYPE_def] \\
+  reverse conj_tac >- (EVAL_TAC \\ simp[]) \\
+  xlet_auto >- xsimpl \\
+  xlet_auto >- xsimpl \\
+  rename [‘W8ARRAY bv (REPLICATE 9 0w)’] \\
+  xlet ‘POSTv uv. &UNIT_TYPE () uv * W8ARRAY bv (0w :: n2w8 ((t+d) DIV 1000)) *
+        TIME <| latest_time := t+d; microseconds_elapsed := ds|>’
+  >- (qpat_abbrev_tac `Q = $POSTv _` >>
+      simp [ts_ffi_part_def, TIME_def, IOx_def, IO_def] >>
+      xpull >> qunabbrev_tac `Q` >>
+      xffi \\ xsimpl \\
+      simp[TIME_def,IOx_def,ts_ffi_part_def,mk_ffi_next_def,IO_def] \\
+      qmatch_goalsub_abbrev_tac `FFI_part st f ns` \\
+      CONV_TAC(RESORT_EXISTS_CONV List.rev) \\
+      map_every qexists_tac[‘events’, ‘ns’, ‘f’, ‘st’] \\
+      simp[Abbr‘f’,Abbr‘st’,Abbr‘ns’,mk_ffi_next_def,ffi_get_now_milliseconds_def,getNowMilliseconds_def] \\ xsimpl \\
+      qpat_abbrev_tac ‘new_events = events ++ _’ \\
+      qexists ‘new_events’ \\ xsimpl) \\
+  xlet_auto >- xsimpl \\
+  xlet_auto >- (xsimpl \\ map_every qexists_tac [‘t’, ‘d’] \\ fs[]) \\
+  xlet ‘POSTv boolv. W8ARRAY bv (0w::n2w8 ((d + t) DIV 1000)) * TIME  <|latest_time := d + t; microseconds_elapsed := ds|> * &BOOL T boolv’
+  >- (xapp_spec eq_word8_v_thm \\ xsimpl \\ fs[BOOL_def] \\ metis_tac []) \\
+  xif \\ qexists ‘T’ \\ fs[] \\
+  xapp \\ xsimpl \\ fs[LENGTH_n2w8] \\
+  qpat_abbrev_tac ‘new_latest_time = (d + t) DIV 1000’ \\
+  fs[n2w8_def] \\ qspec_then ‘new_latest_time’ mp_tac n2w8_def \\
+  simp[] \\ DISCH_THEN (SUBST1_TAC o SYM) \\ simp[w82n_n2w8]
+QED
+
+val _ = export_theory();
